theories/models/utp_vdm_simple/utp_vdm_types.thy
@@ -83,7 +83,7 @@ syntax
   "_vty_map_to"  :: "vty \<Rightarrow> vty \<Rightarrow> vty" ("@map _ to _")
   "_vty_seq1_of" :: "vty \<Rightarrow> vty" ("@seq1 of _")
   "_vty_prod"    :: "vty \<Rightarrow> vty \<Rightarrow> vty" (infixl "\<times>" 20)
-  "_vty_quo"     :: "vty \<Rightarrow> 'a set" ("\<parallel>_\<parallel>\<^sub>t")
+  "_vty_quo"     :: "vty \<Rightarrow> 'a set" ("\<parallel>_\<parallel>")
   "_vty_inv"     :: "vty \<Rightarrow> pttrn \<Rightarrow> pexpr \<Rightarrow> vty" ("_ inv _ == _")
   "_vty_collect" :: "pexpr \<Rightarrow> pexpr \<Rightarrow> vty" ("(1{_|/ _})")
   "_vty_decl"    :: "('a, 'm) PVAR \<Rightarrow> vty \<Rightarrow> vty_decl" (infix ":" 50)
@@ -113,14 +113,14 @@ translations
   "_vty_collect v P" == "CONST CollectD v P"
 
 
-term "\<parallel>@seq1 of @char\<parallel>\<^sub>t"
+term "\<parallel>@seq1 of @char\<parallel>"
 
-term "\<parallel>@map @char to @int\<parallel>\<^sub>t"
+term "\<parallel>@map @char to @int\<parallel>"
 
 (* term "`x := \<langle><1>\<rangle> : @seq1 of @nat1`" *)
 
-term "\<parallel>{($x : @int,$y : @int) | $x = $y}\<parallel>\<^sub>t"
+term "\<parallel>{($x : @int,$y : @int) | $x = $y}\<parallel>"
 
-term "\<parallel>[\<langle>1\<rangle>] : @seq1 of @int\<parallel>"
+term "|[\<langle>1\<rangle>] : @seq1 of @int|"
 
 end
