theories/tactics/utp_subst_tac.thy
@@ -1,0 +1,35 @@
+(******************************************************************************)
+(* Project: Unifying Theories of Programming                                  *)
+(* File: utp_subst_tac.thy                                                    *)
+(* Author: Simon Foster, University of York (UK)                              *)
+(******************************************************************************)
+
+header {* Proof Tactic for Substitution *}
+
+theory utp_subst_tac
+imports "../laws/utp_subst_laws"
+begin
+
+ML {*
+  fun utp_subst_simpset ctxt =
+    (simpset_of ctxt)
+      addsimps (usubst.get ctxt)
+      addsimps (closure.get ctxt)
+      addsimps (typing.get ctxt)
+      addsimps (defined.get ctxt);
+*}
+
+ML {*
+  fun utp_subst_tac thms ctxt i =
+    CHANGED (
+      TRY (asm_full_simp_tac (utp_subst_simpset ctxt) i))
+*}
+
+
+method_setup utp_subst_tac = {*
+  Attrib.thms >>
+  (fn thms => fn ctxt =>
+    SIMPLE_METHOD' (utp_subst_tac thms ctxt))
+*} "proof tactic for substitution"
+
+end
